towards negative soundness

theories/Decidability/NegativeSoundness.v
@@ -1,9 +1,10 @@
 (** * LogRel.Decidability.NegativeSoundness: implementation failure implies negation of typing. *)
 From Coq Require Import Nat Lia Arith.
 From Equations Require Import Equations.
-From LogRel.AutoSubst Require Import core unscoped Ast Extra.
-From LogRel Require Import Utils BasicAst Context Notations UntypedReduction DeclarativeTyping DeclarativeInstance GenericTyping NormalForms Weakening.
-From LogRel Require Import Validity LogicalRelation Fundamental DeclarativeSubst TypeConstructorsInj DeclarativeNeutralConv AlgorithmicTyping BundledAlgorithmicTyping Normalisation AlgorithmicConvProperties AlgorithmicTypingProperties.
+From LogRel Require Import Syntax.All GenericTyping DeclarativeTyping AlgorithmicTyping.
+From LogRel.TypingProperties Require Import PropertiesDefinition DeclarativeProperties SubstConsequences TypeConstructorsInj NeutralConvProperties.
+From LogRel.Algorithmic Require Import BundledAlgorithmicTyping AlgorithmicConvProperties AlgorithmicTypingProperties.
+From LogRel Require Import Utils.
 
 From LogRel.Decidability Require Import Functions Soundness Completeness.
 From PartialFun Require Import Monad PartialFun MonadExn.
@@ -12,480 +13,6 @@ Set Universe Polymorphism.
 Set Printing Primitive Projection Parameters.
 
 Import DeclarativeTypingProperties.
-
-Definition nat_hd_view (Γ : context) {t t' : term} (nft : isNat t) (nft' : isNat t') : Type :=
-  match nft, nft' with
-    | ZeroNat, ZeroNat => True
-    | @SuccNat u, @SuccNat u' => [Γ |-[de] u ≅ u' : tNat]
-    | NeNat _, NeNat _ => [Γ |-[de] t ~ t' : tNat ]
-    | _, _ => False
-  end.
-
-
-Lemma nat_conv_inj : forall (Γ : context) (t t' : term) (nft : isNat t) (nft' : isNat t'),
-  [Γ |-[de] t ≅ t' : tNat] ->
-  nat_hd_view Γ nft nft'.
-Proof.
-  intros * Hconv.
-  eapply Fundamental in Hconv as [HΓ Hnat _ _ Hconv].
-  eapply Escape.reducibleTmEq in Hconv.
-  unshelve eapply Irrelevance.LRTmEqIrrelevant' in Hconv ; try reflexivity.
-  2: now eapply Nat.natRed, Properties.soundCtx.
-  1: exact one.
-  clear Hnat.
-  cbn in *.
-  set (nRed := {| NatRedTy.red := redtywf_refl (wft_term (ty_nat (Properties.soundCtx HΓ))) |}) in *.
-  clearbody nRed.
-
-  revert nft nft'.
-  pattern t, t', Hconv.
-  unshelve eapply NatRedTmEq.NatRedTmEq_mut_rect ; clear t t' Hconv.
-  
-  - exact (fun n n' _ => forall (nft : isNat n) (nft' : isNat n'), nat_hd_view Γ nft nft').
-  
-  - cbn.
-    intros t u t' u' [_ redt%redtm_sound] [_ redu%redtm_sound] ? _ IH Ht Hu.
-    eapply red_whnf in redt as ->, redu as ->.
-    2-3: gen_typing.
-    eauto.
-
-  - cbn.
-    intros nft nft'.
-    rewrite (isNat_zero nft), (isNat_zero nft') ; cbn.
-    easy.
-
-  - cbn.
-    intros ?? [] _ nft nft'.
-    rewrite (isNat_succ _ nft), (isNat_succ _ nft') ; cbn.
-    eapply convtm_exp ; gen_typing.
-
-  - cbn.
-    intros ?? [] nft nft' ; refold.
-    epose proof (isNat_ne _ nft) as [? ->].
-    1: now eapply conv_neu_ne in conv.
-    epose proof (isNat_ne _ nft') as [? ->].
-    1: now eapply conv_neu_ne in conv.
-    cbn.
-    assumption.
-
-Qed.
-
-Definition univ_hd_view (Γ : context) {T T' : term} (nfT : isType T) (nfT' : isType T') : Type :=
-  match nfT, nfT' with
-    | @UnivType s, @UnivType s' => False
-    | @ProdType A B, @ProdType A' B' => [Γ |-[de] A' ≅ A : U] × [Γ,, A' |-[de] B ≅ B' : U]
-    | NatType, NatType => True
-    | EmptyType, EmptyType => True
-    | NeType _, NeType _ => [Γ |- T ~ T' : U]
-    | @SigType A B, @SigType A' B' => [Γ |-[de] A ≅ A' : U] × [Γ,, A |-[de] B ≅ B' : U]
-    | @IdType A x y, @IdType A' x' y' => [× [Γ |-[de] A ≅ A' : U], [Γ |-[de] x ≅ x' : A] & [Γ |-[de] y ≅ y' : A]]
-    | _, _ => False
-  end.
-
-Lemma escapeEqzero {Γ A B} (lr : [Γ ||-< zero > A]) :
-    [Γ |- A : U] ->
-    [Γ |- B : U] ->
-    [ Γ ||-< zero > A ≅ B | lr ] ->
-    [Γ |- A ≅ B : U].
-Proof.
-  remember zero as l eqn:e.
-  revert e B.
-  pattern l, Γ, A, lr ; eapply Induction.LR_rect_TyUr.
-  all: clear.
-  + intros ??? [? lt] -> **.
-    inversion lt.
-  + intros ??? [] -> ??? [].
-    cbn in *.
-    etransitivity.
-    1: eapply RedConvTeC, subject_reduction ; gen_typing.
-    etransitivity.
-    1: gen_typing.
-    symmetry.
-    eapply RedConvTeC, subject_reduction ; gen_typing.
-
-  + intros ??? [dom cod] * IHdom IHcod -> ??? [dom' cod' ??? [shpRed posRed]] ; cbn in *.
-    assert [Γ |- A ⤳* tProd dom cod : U].
-    {
-      eapply subject_reduction ; gen_typing.
-    }
-    assert [Γ |- tProd dom cod : U] as [? [? [[-> ??] _]]%termGen']%dup
-      by boundary.
-    assert [Γ |- B ⤳* tProd dom' cod' : U].
-    {
-      eapply subject_reduction ; gen_typing.
-    }
-    assert [Γ |- tProd dom' cod' : U] as [? [? [[-> ??] _]]%termGen']%dup
-      by boundary.
-    eapply convtm_exp ; tea.
-    1-2: repeat econstructor ; boundary.
-
-    assert [Γ |-[de] dom ≅ dom' : U].
-    {
-      erewrite <- (wk_id_ren_on Γ dom).
-      unshelve eapply IHdom ; eauto.
-      - boundary.
-      - now rewrite wk_id_ren_on.
-      - erewrite <- (wk_id_ren_on Γ dom').
-        eapply shpRed.
-    }
-
-    assert [Γ,, dom |-[ de ] cod ≅ cod' : U].
-    {
-      unshelve epose proof (IHcod _ _ _ _ (Neutral.var0 _ _ _)) as IHcod'.
-      1: eapply wk1.
-      3: rewrite wk1_ren_on ; reflexivity.
-      1: econstructor ; [boundary|..].
-      1-2: now econstructor.
-      cbn in *.
-      replace cod[_] with cod in IHcod'.
-      2:{
-        clear.
-        bsimpl.
-        rewrite scons_eta'.
-        now bsimpl.
-      }
-      eapply IHcod' ; eauto.
-      1: eapply stability1 ; tea.
-      1-2: constructor ; boundary.
-      unshelve epose proof (posRed _ _ _ _ (Neutral.var0 _ _ _)) as posRed'.
-      1: eapply wk1.
-      3: rewrite wk1_ren_on ; reflexivity.
-      1: econstructor ; [boundary|..].
-      1-2: now econstructor.
-      cbn in *.
-      replace cod'[_] with cod' in posRed'.
-      2:{
-        clear.
-        bsimpl.
-        rewrite scons_eta'.
-        now bsimpl.
-      }
-      Irrelevance.irrelevance.
-    }
-
-    now constructor.
-
-  + intros ??? [] -> ??? [].
-    etransitivity.
-    1: eapply RedConvTeC, subject_reduction ; gen_typing.
-    etransitivity.
-    1: gen_typing.
-    symmetry.
-    eapply RedConvTeC, subject_reduction ; gen_typing.
-
-  + intros ??? [] -> ??? [].
-    etransitivity.
-    1: eapply RedConvTeC, subject_reduction ; gen_typing.
-    etransitivity.
-    1: gen_typing.
-    symmetry.
-    eapply RedConvTeC, subject_reduction ; gen_typing.
-
-  + intros ??? [dom cod] * IHdom IHcod -> ??? [dom' cod' ??? [shpRed posRed]] ; cbn in *.
-    assert [Γ |- A ⤳* tSig dom cod : U].
-    {
-      eapply subject_reduction ; gen_typing.
-    }
-    assert [Γ |- tSig dom cod : U] as [? [? [[-> ??] _]]%termGen']%dup
-      by boundary.
-    assert [Γ |- B ⤳* tSig dom' cod' : U].
-    {
-      eapply subject_reduction ; gen_typing.
-    }
-    assert [Γ |- tSig dom' cod' : U] as [? [? [[-> ??] _]]%termGen']%dup
-      by boundary.
-    eapply convtm_exp ; tea.
-    1-2: repeat econstructor ; boundary.
-
-    assert [Γ |-[de] dom ≅ dom' : U].
-    {
-      erewrite <- (wk_id_ren_on Γ dom).
-      unshelve eapply IHdom ; eauto.
-      - boundary.
-      - now rewrite wk_id_ren_on.
-      - erewrite <- (wk_id_ren_on Γ dom').
-        eapply shpRed. 
-    }
-
-    assert [Γ,, dom |-[ de ] cod ≅ cod' : U].
-    {
-      unshelve epose proof (IHcod _ _ _ _ (Neutral.var0 _ _ _)) as IHcod'.
-      1: eapply wk1.
-      3: rewrite wk1_ren_on ; reflexivity.
-      1: econstructor ; [boundary|..].
-      1-2: now econstructor.
-      cbn in *.
-      replace cod[_] with cod in IHcod'.
-      2:{
-        clear.
-        bsimpl.
-        rewrite scons_eta'.
-        now bsimpl.
-      }
-      eapply IHcod' ; eauto.
-      1: eapply stability1 ; tea.
-      1-2: constructor ; boundary.
-      unshelve epose proof (posRed _ _ _ _ (Neutral.var0 _ _ _)) as posRed'.
-      1: eapply wk1.
-      3: rewrite wk1_ren_on ; reflexivity.
-      1: econstructor ; [boundary|..].
-      1-2: now econstructor.
-      cbn in *.
-      replace cod'[_] with cod' in posRed'.
-      2:{
-        clear.
-        bsimpl.
-        rewrite scons_eta'.
-        now bsimpl.
-      }
-      Irrelevance.irrelevance.
-    }
-
-    now constructor.
-
-  + intros ??? [T x y outTy ?] IH ? -> ??? [T' x' y' outTy' ? eq']; cbn in *.
-    subst outTy outTy' ; cbn in *.
-    assert [Γ |- A ⤳* tId T x y : U].
-    {
-      eapply subject_reduction ; gen_typing.
-    }
-    assert [Γ |- tId T x y : U] as [? [? [[-> ??] _]]%termGen']%dup
-      by boundary.
-    assert [Γ |- B ⤳* tId T' x' y' : U].
-    {
-      eapply subject_reduction ; gen_typing.
-    }
-    assert [Γ |- tId T' x' y' : U] as [? [? [[-> ??] _]]%termGen']%dup
-      by boundary.
-    cbv in eq' ; refold.
-    eapply convtm_exp ; tea.
-    1-2: repeat econstructor ; boundary.
-    econstructor ; tea.
-    * now eapply IH.
-    * now Escape.escape.
-    * now Escape.escape.
-
-Qed.
-
-Theorem univ_conv_inj : forall (Γ : context) (T T' : term) (nfT : isType T) (nfT' : isType T'),
-  [Γ |-[de] T ≅ T' : U] ->
-  univ_hd_view Γ nfT nfT'.
-Proof.
-  intros * Hconv.
-  assert [Γ |- T : U] as HT by boundary.
-  assert [Γ |- T' : U] as HT' by boundary.
-  revert HT HT'. 
-  eapply Fundamental in Hconv as [HΓ HU HT HT' Hconv].
-  eapply Escape.reducibleTmEq in Hconv.
-  eapply Escape.reducibleTm in HT, HT'.
-  set (HTred := Escape.reducibleTy _ HU) in *.
-  clearbody HTred.
-  clear HU.
-  eapply Universe.univTmTy in HT, HT' ; cbn.
-  unshelve eapply Universe.univEqTmEqTy in Hconv ; [idtac|eassumption|..].
-  destruct (Induction.invLRU HTred) as [? lt ? ?] ; cbn in *.
-  inversion lt ; subst ; clear - HT Hconv.
-
-  revert HT nfT T' nfT' Hconv.
-  generalize (eq_refl : zero = zero).
-  generalize zero at 1 3; intros l eql HT; revert eql.
-
-  pattern l, Γ, T, HT; apply Induction.LR_rect_TyUr; clear l Γ T HT.
-  all: intros ? Γ T.
-  
-  - intros [? lt] -> **.
-    now inversion lt.
-
-  - intros [nT ? ne] -> nfT T' nfT' [nT' ? ne'] HT HT' ; cbn in *.
-    assert (T = nT) as <- by
-      (apply red_whnf ; gen_typing).
-    assert (T' = nT') as <- by
-      (apply red_whnf ; gen_typing).
-    destruct nfT.
-    1-6: apply convneu_whne in ne; inversion ne.
-    destruct nfT'.
-    1-6: symmetry in ne'; apply convneu_whne in ne'; inversion ne'.
-    cbn. easy.
-
-  - intros [dom cod red] _ _ -> nfT T' nfT' [dom' cod' red'] HT HT' ; cbn in *.
-    assert (T = tProd dom cod) as HeqT by (apply red_whnf ; gen_typing). 
-    assert (T' = tProd dom' cod') as HeqT' by (apply red_whnf ; gen_typing).
-    destruct nfT; cycle -1.
-    1: subst ; exfalso ; gen_typing.
-    all: try congruence.
-    destruct nfT'; cycle -1.
-    1: subst ; exfalso ; gen_typing.
-    all: try congruence.
-    inversion HeqT ; inversion HeqT' ; subst ; clear HeqT HeqT'; cbn.
-    edestruct (Poly.polyRedEqId _ polyRed0) ; cbn in *.
-    eapply termGen' in HT as [? [[]]].
-    eapply termGen' in HT' as [? [[]]].
-    assert [Γ |- dom' ≅ dom : U] by
-      (symmetry ; now eapply escapeEqzero).
-    split ; tea.
-    eapply stability1.
-    3: now constructor.
-    1-2: boundary.
-    eapply escapeEqzero ; tea.
-    eapply stability1 ; tea.
-    all: boundary. 
-      
-  - intros [] -> nfT T' nfT' [] ??.
-    assert (T' = tNat) as HeqT' by (eapply redtywf_whnf ; gen_typing).
-    assert (T = tNat) as HeqT by (eapply redtywf_whnf ; gen_typing).
-    destruct nfT; inversion HeqT.
-    + destruct nfT'; inversion HeqT'.
-      * constructor.
-      * exfalso; subst; inversion w.
-    + exfalso; subst; inversion w.
-
-  - intros [] -> nfT T' nfT' [] ??.
-    assert (T' = tEmpty) as HeqT' by (eapply redtywf_whnf ; gen_typing).
-    assert (T = tEmpty) as HeqT by (eapply redtywf_whnf ; gen_typing).
-    destruct nfT; inversion HeqT.
-    + destruct nfT'; inversion HeqT'.
-      * econstructor.
-      * exfalso; subst; inversion w.
-    + exfalso; subst; inversion w.
-
-  - intros [dom cod red] _ _ -> nfT T' nfT' [dom' cod' red'] ?? ; cbn in *.
-    assert (T = tSig dom cod) as HeqT by (apply red_whnf ; gen_typing).
-    assert (T' = tSig dom' cod') as HeqT' by (apply red_whnf ; gen_typing).
-    destruct nfT; cycle -1.
-    1: subst; inv_whne.
-    all: try congruence.
-    destruct nfT'; cycle -1.
-    1: subst; inv_whne.
-    all: try congruence.
-    inversion HeqT ; inversion HeqT' ; subst ; clear HeqT HeqT'; cbn.
-    eapply Poly.polyRedEqId in polyRed0 as [].
-    eapply termGen' in HT as [? [[]]].
-    eapply termGen' in HT' as [? [[]]].
-    assert [Γ |- dom ≅ dom' : U] by now eapply escapeEqzero.
-    split ; tea.
-    eapply escapeEqzero ; tea.
-    eapply stability1 ; tea.
-    all: boundary.
-
-  - intros [??? ty] _ _ -> nfT T' nfT' [??? ty'] ?? ; cbn in *.
-    assert (T = ty) as HeqT by (apply red_whnf; gen_typing).
-    assert (T' = ty') as HeqT' by (apply red_whnf; gen_typing).
-    destruct nfT; cycle -1; [subst; inv_whne|..]; unfold ty in *; try congruence.
-    destruct nfT'; cycle -1; [subst; inv_whne|..]; unfold ty' in *; try congruence.
-    cbn; inversion HeqT; inversion HeqT'; subst ; clear HeqT HeqT' ; cbn in *.
-    eapply termGen' in HT as [? [[]]].
-    eapply termGen' in HT' as [? [[]]].
-    split.
-    2-3: now Escape.escape.
-    now eapply escapeEqzero.
-Qed.
-
-Lemma empty_conv_inj (Γ : context) (t t' : term) :
-  whne t -> whne t' ->
-  [Γ |-[de] t ≅ t' : tEmpty] ->
-  [Γ |-[de] t ~ t' : tEmpty].
-Proof.
-  intros * wt wt' Hconv.
-  eapply Fundamental in Hconv as [HΓ Hemp _ _ Hconv].
-  eapply Escape.reducibleTmEq in Hconv.
-  unshelve eapply Irrelevance.LRTmEqIrrelevant' in Hconv ; try reflexivity.
-  2: now eapply Empty.emptyRed, Properties.soundCtx.
-  1: exact one.
-  clear Hemp.
-  cbn in *.
-  set (nRed := {| EmptyRedTy.red := redtywf_refl (wft_term (ty_empty (Properties.soundCtx HΓ))) |}) in *.
-  clearbody nRed.
-
-  destruct Hconv as [?? ?? redL redR ? Hp].
-  inversion Hp as [?? []]; subst.
-  erewrite red_whnf.
-  2: eapply redtm_sound, redR.
-  2: now econstructor.
-  erewrite (red_whnf t).
-  2: eapply redtm_sound, redL.
-  2: now econstructor.
-
-  assumption.
-
-Qed.
-
-Definition id_hd_view (Γ : context) (A x x' : term) {t t' : term} (nft : isId t) (nft' : isId t') : Type :=
-  match nft, nft' with
-    | @ReflId A a, @ReflId A' a' => [Γ |- A ≅ A'] × [Γ |- a ≅ a' : A]
-    | NeId _, NeId _ => [Γ |- t ~ t' : tId A x x']
-    | _, _ => False
-  end.
-
-Lemma id_conv_inj : forall (Γ : context) (A x y t t' : term) (nft : isId t) (nft' : isId t'),
-  [Γ |-[de] t ≅ t' : tId A x y] ->
-  id_hd_view Γ A x y nft nft'.
-Proof.
-  intros * Hconv.
-  eapply Fundamental in Hconv as [HΓ Hid _ _ Hconv].
-  eapply Escape.reducibleTmEq in Hconv.
-  set (HTred := Escape.reducibleTy _ Hid) in *.
-  clearbody HTred.
-  clear Hid.
-  unshelve eapply Irrelevance.LRTmEqIrrelevant' in Hconv ; try reflexivity.
-  1: exact one.
-  1: now eapply LRId', Induction.invLRId.
-  cbn in *.
-  clear - Hconv.
-  
-  destruct Hconv as [u u' ? ? _ p] ; cbn in *.
-  assert (t = u) as <- by (eapply red_whnf ; gen_typing).
-  assert (t' = u') as <- by (eapply red_whnf ; gen_typing).
-  destruct p as [? | ? ? []] ; cbn in *.
-
-  - Escape.escape.
-    rewrite (isId_refl _ _ nft), (isId_refl _ _ nft') ; cbn.
-    split.
-    + etransitivity ; eauto.
-      now symmetry.
-    + econstructor ; eauto.
-      etransitivity ; eauto.
-      now symmetry.
-
-  - edestruct (isId_ne ne) as [? ->] ; [now eapply conv_neu_ne in conv |..].
-    edestruct (isId_ne ne') as [? ->] ; [now eapply conv_neu_ne in conv |..].
-    cbn.
-    unfold IdRedTyPack.outTy in conv ; cbn in *.
-    destruct (Id.IdRedTy_inv (Induction.invLRId HTred)) as [eA ex ey].
-    rewrite <- eA, <- ex, <- ey in conv.
-    assumption.
-
-Qed.
-
-Lemma neu_conv_inj (Γ : context) (A t t' : term) :
-  whne A -> whne t -> whne t' ->
-  [Γ |-[de] t ≅ t' : A] ->
-  [Γ |-[de] t ~ t' : A].
-Proof.
-  intros * wA wt wt' Hconv.
-  eapply Fundamental in Hconv as [HΓ Hne _ _ Hconv].
-  eapply Escape.reducibleTmEq in Hconv.
-  unshelve eapply Irrelevance.LRTmEqIrrelevant' in Hconv ; try reflexivity.
-  1: exact one.
-  1:{
-    eapply Neutral.neu.
-    2: eapply conv_neu_refl, neutral_ty_inv ; tea.
-    all: now eapply Escape.escapeTy.
-  }
-  cbn in *.
-
-  destruct Hconv as [?? redL redR ?] ; cbn in *.
-  erewrite red_whnf.
-  2: eapply redtm_sound, redR.
-  2: now econstructor.
-  erewrite (red_whnf t).
-  2: eapply redtm_sound, redL.
-  2: now econstructor.
-
-  assumption.
-
-Qed.
-
-Import DeclarativeTypingProperties AlgorithmicTypingProperties.
 
 Lemma ty_mismatch_hd_view Γ T V (tT : isType T) (tV : isType V) :
   build_nf_ty_view2 T V = ty_mismatch T V ->
@@ -531,7 +58,7 @@ Proof.
     all: destruct n0 ; cbn ; try solve [intros [=]].
     all: unshelve (intros _ ; left ; do 2 eexists).
     all: try solve [constructor].
-    1-8: econstructor ; eapply whne_can ; tea ; solve [now apply zip_can | intros c ; inversion c].
+    1-8: econstructor ; eapply not_can_whne ; tea ; solve [now apply zip_can | intros c ; inversion c].
     all: now cbn.
 
   - destruct (build_nf_view1 t), (build_nf_view1 u) ; cbn.
@@ -544,7 +71,7 @@ Proof.
     all: split ; [reflexivity|..].
     Unshelve.
     all: try solve [constructor].
-    5-8: econstructor ; eapply whne_can ; tea ; solve [now apply zip_can | intros c ; inversion c].
+    5-8: econstructor ; eapply not_can_whne ; tea ; solve [now apply zip_can | intros c ; inversion c].
     all: now cbn.
     
   - unshelve erewrite whne_ty_view1 ; tea ; cbn.
@@ -553,7 +80,7 @@ Proof.
 
 Qed.
 
-Lemma prod_tm_inj Γ A B A' B' :
+Lemma prod_tm_inj `{TermConstructorsInj (ta := de)} Γ A B A' B' :
   [Γ |-[de] tProd A B ≅ tProd A' B' : U] ->
   [Γ |-[de] A' ≅ A : U] × [Γ,,A' |-[de] B ≅ B' : U].
 Proof.
@@ -562,7 +89,7 @@ Proof.
   now cbn in *.
 Qed.
 
-Lemma sig_tm_inj Γ A B A' B' :
+Lemma sig_tm_inj `{TermConstructorsInj (ta := de)} Γ A B A' B' :
   [Γ |-[de] tSig A B ≅ tSig A' B' : U] ->
   [Γ |-[de] A ≅ A' : U] × [Γ,,A |-[de] B ≅ B' : U].
 Proof.
@@ -571,7 +98,7 @@ Proof.
   now cbn in *.
 Qed.
 
-Lemma id_tm_inj Γ A x y A' x' y' :
+Lemma id_tm_inj `{TermConstructorsInj (ta := de)} Γ A x y A' x' y' :
   [Γ |-[de] tId A x y ≅ tId A' x' y' : U] ->
   [× [Γ |-[de] A ≅ A' : U], [Γ |-[de] x ≅ x' : A] & [Γ |-[de] y ≅ y' : A]].
 Proof.
@@ -580,483 +107,420 @@ Proof.
   now cbn in *.
 Qed.
 
-#[universes(polymorphic)]Definition conv_sound_type
-    (x : conv_full_dom)
-    (r : conv_full_cod x) : Type :=
-  match x, r with
-  | (ty_state;Γ;_;T;V), (success _) =>  [Γ |-[al] T ≅ V]
-  | (ty_red_state;Γ;_;T;V), (success _) => [Γ |-[al] T ≅h V]
-  | (tm_state;Γ;A;t;u), (success _) => [Γ |-[al] t ≅ u : A]
-  | (tm_red_state;Γ;A;t;u), (success _) =>
-      whnf A -> whnf t -> whnf u -> [Γ |-[al] t ≅h u : A]
-  | (ne_state;Γ;_;m;n), (success T) => [Γ |-[al] m ~ n ▹ T]
-  | (ne_red_state;Γ;_;m;n), (success T) => [Γ |-[al] m ~h n ▹ T] × whnf T
-  
-  | (ty_state;Γ;_;T;V), (exception _) => ~ [Γ |-[de] T ≅ V]
-  | (ty_red_state;Γ;_;T;V), (exception _) => ~ [Γ |-[de] T ≅ V]
-  | (tm_state;Γ;A;t;u), (exception _) => ~ [Γ |-[de] t ≅ u : A]
-  | (tm_red_state;Γ;A;t;u), (exception _) => ~ [Γ |-[de] t ≅ u : A]
-  | (ne_state;Γ;_;m;n), (exception _) => ~ ∑ T, [Γ |-[de] m ~ n : T]
-  | (ne_red_state;Γ;_;m;n), (exception _) => ~ ∑ T, ([Γ |-[de] m ~ n : T] × whnf T)
+Import AlgorithmicTypingProperties.
+
+Section ConvSoundNeg.
+  Context `{!TypingSubst (ta := de)}
+    `{!TypeReductionComplete (ta := de)} `{!TypeConstructorsInj (ta := de)}
+    `{!TermConstructorsInj (ta := de)} `{!ConvNeutralConvPos (ta := de)}.
+
+  #[universes(polymorphic)]Definition conv_sound_type
+      (x : conv_full_dom)
+      (r : conv_full_cod x) : Type :=
+    match x, r with
+    | (ty_state;Γ;_;T;V), (exception _) => ~ [Γ |-[de] T ≅ V]
+    | (ty_red_state;Γ;_;T;V), (exception _) => ~ [Γ |-[de] T ≅ V]
+    | (tm_state;Γ;A;t;u), (exception _) => ~ [Γ |-[de] t ≅ u : A]
+    | (tm_red_state;Γ;A;t;u), (exception _) => ~ [Γ |-[de] t ≅ u : A]
+    | (ne_state;Γ;_;m;n), (exception _) => ~ ∑ T, [Γ |-[de] m ~ n : T]
+    | (ne_red_state;Γ;_;m;n), (exception _) => ~ ∑ T, ([Γ |-[de] m ~ n : T] × whnf T)
+    | _, success _ =>  True
+    end.
+
+  #[universes(polymorphic)]Definition conv_sound_pre
+    (x : conv_full_dom) : Type :=
+  match x with
+  | (ty_state;Γ;_;T;V) => [Γ |-[de] T] × [Γ |-[de] V]
+  | (ty_red_state;Γ;_;T;V) => [× whnf T, whnf V & [Γ |-[de] T] × [Γ |-[de] V]]
+  | (tm_state;Γ;A;t;u) => [Γ |-[de] t : A] × [Γ |-[de] u : A]
+  | (tm_red_state;Γ;A;t;u) => [× whnf A, whnf t, whnf u & [Γ |-[de] t : A] × [Γ |-[de] u : A]]
+  | (ne_state;Γ;_;m;n) => (whne m × whne n) × (well_typed (ta := de) Γ m × well_typed (ta := de) Γ n)
+  | (ne_red_state;Γ;_;m;n) => (whne m × whne n) × (well_typed (ta := de) Γ m × well_typed (ta := de) Γ n)
   end.
 
-#[universes(polymorphic)]Definition conv_sound_pre
-  (x : conv_full_dom) : Type :=
-match x with
-| (ty_state;Γ;_;T;V) => [Γ |-[de] T] × [Γ |-[de] V]
-| (ty_red_state;Γ;_;T;V) => [× whnf T, whnf V & [Γ |-[de] T] × [Γ |-[de] V]]
-| (tm_state;Γ;A;t;u) => [Γ |-[de] t : A] × [Γ |-[de] u : A]
-| (tm_red_state;Γ;A;t;u) => [× whnf A, whnf t, whnf u & [Γ |-[de] t : A] × [Γ |-[de] u : A]]
-| (ne_state;Γ;_;m;n) => [× (* whne m, whne n,*) well_typed (ta := de) Γ m & well_typed (ta := de) Γ n]
-| (ne_red_state;Γ;_;m;n) => [× (* whne m, whne n, *) well_typed (ta := de) Γ m & well_typed (ta := de) Γ n]
-end.
 
-
-
-Lemma _implem_conv_neg_sound :
-  funrect _conv conv_sound_pre conv_sound_type.
-Proof.
-  intros x pre.
-  funelim (_conv x) ; cbn in pre |- *.
-  
-  6: simp conv_ne_red ; cbn.
-  5: simp conv_ne ; destruct (build_ne_view2 _ _) eqn:e ; cbn ; try easy.
-  4: simp conv_tm_red ; destruct (build_nf_view3 _ _ _) as [??? [] | | | | | | | | ]  eqn:e ;
-    cbn ; try easy.
-  3: simp conv_tm ; cbn.
-  2: simp conv_ty_red ; cbn ; destruct (build_nf_ty_view2 _ _) eqn:e ; cbn.
-  1: simp conv_ty ; cbn.
-  
-  - intros T' []%red_sound V' []%red_sound.
-    eapply typeConvRed_prem2 in pre as [[] Hpost2]%dup ; tea.
-    split ; [split|..] ; tea.
-    intros [|] Hnty ; cbn.
-    1: now econstructor.
-    intros Hty.
-    eapply Hnty.
-    etransitivity.
-    2: etransitivity ; tea.
-    1: symmetry. 
-    all: eapply RedConvTyC, subject_reduction_type ; eauto.
-    all: boundary.
-
-  - destruct s1, s2 ; now constructor. 
-
-  - destruct pre as [_ _ [pre [[]]%typePiCongAlg_prem0%dup]%dup].
-    split ; [easy|..].
-    intros [|] Hty ; cbn.
-    2: now intros []%prod_ty_inj.
-    eapply dup in Hty as [Hty ?%algo_conv_sound] ; tea.
-    eapply dup in pre as [pre ?%typePiCongAlg_prem1] ; tea.
-    split ; [easy|..].
-    intros [|] Hty'.
-    2:{
-      intros []%prod_ty_inj.
-      eapply Hty', stability1 ; eassumption.
-    }
-    now econstructor.
-
-  - now econstructor.
-  
-  - now econstructor.
-  
-  - destruct pre as [_ _ [pre [[]]%typeSigCongAlg_prem0%dup]%dup].
-    split ; [easy|..].
-    intros [|] Hty ; cbn.
-    2: now intros []%sig_ty_inj.
-    eapply dup in Hty as [Hty ?%algo_conv_sound] ; tea.
-    eapply dup in pre as [pre ?%typeSigCongAlg_prem1] ; tea.
-    split ; [easy|..].
-    intros [|] Hty'.
-    2: now intros []%sig_ty_inj.
-    now econstructor.
-  
-  - destruct pre as [_ _ [pre [[]]%typeIdCongAlg_prem0%dup]%dup].
-    split ; [easy|..].
-    intros [|] Hty ; cbn.
-    2: now intros [? _]%id_ty_inj.
-    eapply dup in Hty as [Hty ?%algo_conv_sound] ; tea.
-    eapply dup in pre as [pre [[]]%typeIdCongAlg_prem1%dup] ; tea.
-    split ; [easy|..].
-    intros [|] Hty' ; cbn.
-    2: now intros []%id_ty_inj.
-    eapply dup in Hty' as [Hty' ?%algo_conv_sound] ; tea.
-    eapply dup in pre as [pre ?%typeIdCongAlg_prem2] ; tea.
-    split ; [easy|..].
-    intros [|] Hty'' ; cbn.
-    2: now intros []%id_ty_inj.
+  Lemma _implem_conv_neg_sound :
+    funrect _conv conv_sound_pre conv_sound_type.
+  Proof.
+    intros x pre.
+    funelim (_conv x) ; cbn in pre |- *.
     
-    now econstructor.
-
-  - eapply ty_view2_neutral_can in e as [].
-    destruct pre as [?%whne_can ?%whne_can pre] ; tea.
-    eapply dup in pre as [pre [[]]%typeNeuConvAlg_prem2%dup] ; tea.
-    split ; [easy|..].
-    intros [|] Hty ; cbn.
-    1: now econstructor.
-    unshelve eintros Hty'%ty_conv_inj.
-    1-2: now econstructor.
-    cbn in Hty'.
-    unshelve eapply univ_conv_inj in Hty'.
-    1-2: now econstructor.
-    cbn in Hty'.
-    eauto.
-
-  - destruct pre as [wt wu [Ht Hu]].
-    eapply type_isType in Ht, Hu ; tea.
-    unshelve eapply ty_mismatch_hd_view in e ; tea.
-    unshelve eintros H_view%ty_conv_inj ; tea.
-    rewrite e in H_view.
-    eassumption.
-
-  - easy.
-
-  - intros ? []%red_sound ? []%red_sound ? []%red_sound.
-    eapply termConvRed_prem3 in pre as [[] Hpost3]%dup ; tea.
-    split ; [split|..] ; tea.
-    intros [|] Hnty ; cbn.
-    1: now econstructor.
-    intros Hty.
-    eapply Hnty.
-    eapply TermConv ; refold.
-    2: eapply RedConvTyC, subject_reduction_type ; eauto ; boundary.
-    etransitivity.
-    2: etransitivity ; [eassumption|..].
-    1: symmetry.
-    all: eapply RedConvTeC, subject_reduction ; [..|eassumption].
-    all: boundary.
-
-  - destruct s.
-    destruct pre as [??? [pre [[]]%termPiCongAlg_prem0%dup]%dup].
-    split ; [easy|..].
-    intros [|] Hty ; cbn.
-    2:now intros []%prod_tm_inj.
-    eapply dup in Hty as [Hty ?%algo_conv_sound] ; tea.
-    eapply dup in pre as [pre ?%termPiCongAlg_prem1] ; tea.
-    split ; [easy|..].
-    intros [|] Hty'.
-    + now econstructor.
-    + intros []%prod_tm_inj.
-      eapply Hty', stability1.
-      4: eassumption.
-      all: econstructor.
-      3: now symmetry.
+    6: simp conv_ne_red ; cbn.
+    5: simp conv_ne ; destruct (build_ne_view2 _ _) eqn:e ; cbn ; try easy.
+    4: simp conv_tm_red ; destruct (build_nf_view3 _ _ _) as [??? [] | | | | | | | | ]  eqn:e ;
+      cbn ; try easy.
+    3: simp conv_tm ; cbn.
+    2: simp conv_ty_red ; cbn ; destruct (build_nf_ty_view2 _ _) eqn:e ; cbn.
+    1: simp conv_ty ; cbn.
+    all: try easy.
+    
+    - intros T' []%red_sound V' []%red_sound.
+      eapply typeConvRed_prem2 in pre as [[] Hpost2]%dup ; tea.
+      split ; [split|..] ; tea.
+      intros [|] _ Hnty ; cbn in *.
+      1: easy.
+      intros Hty.
+      eapply Hnty.
+      etransitivity.
+      2: etransitivity ; tea.
+      1: symmetry. 
+      all: eapply RedConvTyC, subject_reduction_type ; eauto.
       all: boundary.
 
-  - intros.
-    destruct s.
-    now econstructor.
-    
-  - intros.
-    destruct s.
-    now econstructor.
-    
-  - destruct s.
-    destruct pre as [??? [pre [[]]%termSigCongAlg_prem0%dup]%dup].
-    split ; [easy|..].
-    intros [|] Hty ; cbn.
-    2:now intros []%sig_tm_inj.
-    eapply dup in Hty as [Hty ?%algo_conv_sound] ; tea.
-    eapply dup in pre as [pre ?%termSigCongAlg_prem1] ; tea.
-    split ; [easy|..].
-    intros [|] Hty'.
-    + now econstructor.
-    + now intros []%sig_tm_inj.
+    - destruct pre as [_ _ [pre [[]]%typePiCongAlg_prem0%dup]%dup].
+      split ; [easy|..].
+      intros [|] Hty ? ; cbn.
+      2: now intros []%prod_ty_inj.
+      eapply implem_conv_graph, algo_conv_sound in Hty ; cbn in * ; tea.
+      eapply dup in pre as [pre ?%typePiCongAlg_prem1] ; tea.
+      split ; [easy|..].
+      intros [|] _ Hty' ; [easy|..].
+      intros []%prod_ty_inj.
+      eapply Hty', stability1 ; eassumption.
 
-  - destruct s.
-    destruct pre as [??? [pre [[]]%termIdCongAlg_prem0%dup]%dup].
-    split ; [easy|..].
-    intros [|] Hty ; cbn.
-    2:now intros []%id_tm_inj.
-    eapply dup in Hty as [Hty ?%algo_conv_sound] ; tea.
-    eapply dup in pre as [pre [? []]%termIdCongAlg_prem1%dup] ; tea.
-    split ; [easy|..].
-    intros [|] Hty' ; cbn in *.
-    2: now intros []%id_tm_inj.
-    eapply dup in Hty' as [Hty' ?%algo_conv_sound] ; tea.
-    eapply dup in pre as [pre ?%termIdCongAlg_prem2] ; tea.
-    split ; [easy|..].
-    intros [|] Hty'' ; cbn in *.
-    2: now intros []%id_tm_inj.
-    now econstructor.
+    - destruct pre as [_ _ [pre [[]]%typeSigCongAlg_prem0%dup]%dup].
+      split ; [easy|..].
+      intros [|] Hty ? ; cbn in *.
+      2: now intros []%sig_ty_inj.
+      eapply implem_conv_graph, algo_conv_sound in Hty ; tea.
+      eapply dup in pre as [pre ?%typeSigCongAlg_prem1] ; tea.
+      split ; [easy|..].
+      intros [|] ? Hty' ; [easy|..].
+      now intros []%sig_ty_inj.
+    
+    - destruct pre as [_ _ [pre [[]]%typeIdCongAlg_prem0%dup]%dup].
+      split ; [easy|..].
+      intros [|] Hty ? ; cbn.
+      2: now intros [? _]%id_ty_inj.
+      eapply implem_conv_graph, algo_conv_sound in Hty ; tea.
+      eapply dup in pre as [pre [[]]%typeIdCongAlg_prem1%dup] ; tea.
+      split ; [easy|..].
+      intros [|] Hty' ? ; cbn in *.
+      2: now intros []%id_ty_inj.
+      eapply implem_conv_graph, algo_conv_sound in Hty' ; tea.
+      eapply dup in pre as [pre ?%typeIdCongAlg_prem2] ; tea.
+      split ; [easy|..].
+      intros [|] ? Hty'' ; cbn in * ; [easy|..].
+      now intros []%id_ty_inj.
 
-  - destruct pre as [??? [pre [[]]%termNeuConvAlg_prem0%dup]%dup] ; tea.
-    eapply whnf_view3_ty_neutral_can in e as [?%whne_can ?%whne_can] ; tea.
-    split ; [easy|..].
-    intros [|] Hty ; cbn.
-    + econstructor ; tea.
-      gen_typing.
-    + destruct s.
-      unshelve eintros ?%univ_conv_inj.
+    - eapply ty_view2_neutral_can in e as [].
+      destruct pre as [?%not_can_whne ?%not_can_whne pre] ; tea.
+      eapply dup in pre as [pre [[]]%typeNeuConvAlg_prem2%dup] ; tea.
+      split ; [now split|..].
+      intros [|] _ Hty ; cbn in * ; [easy|..].
+      unshelve eintros Hty'%ty_conv_inj.
       1-2: now econstructor.
-      cbn in *.
-      eauto.
+      cbn in Hty'.
+      unshelve eapply conv_neu_conv_p in Hty' ; eauto.
+      gen_typing.
 
-  - destruct s.
-    destruct pre as [_ wt wu [Ht Hu]].
-    eapply wft_term, type_isType in Ht, Hu ; tea.
-    unshelve eapply univ_mismatch_hd_view in e ; tea.
-    unshelve eintros H_view%univ_conv_inj ; tea.
-    rewrite e in H_view.
-    eassumption.
+    - destruct pre as [wt wu [Ht Hu]].
+      eapply type_isType in Ht, Hu ; tea.
+      unshelve eapply ty_mismatch_hd_view in e ; tea.
+      unshelve eintros H_view%ty_conv_inj ; tea.
+      rewrite e in H_view.
+      eassumption.
 
-  - destruct pre as [??? [pre [[]]%termFunConvAlg_prem2%dup]%dup] ; tea.
-    split ; [easy|..].
-    intros [|] Hty ; cbn.
-    + intros _ _ _.
+    - intros ? []%red_sound ? []%red_sound ? []%red_sound.
+      eapply termConvRed_prem3 in pre as [[] Hpost3]%dup ; tea.
+      split ; [split|..] ; tea.
+      intros [|] _ Hnty ; cbn in * ; [easy|..].
+      intros Hty.
+      eapply Hnty.
+      eapply TermConv ; refold.
+      2: eapply RedConvTyC, subject_reduction_type ; eauto ; boundary.
+      etransitivity.
+      2: etransitivity ; [eassumption|..].
+      1: symmetry.
+      all: eapply RedConvTeC, subject_reduction ; [..|eassumption].
+      all: boundary.
+
+    - destruct s.
+      destruct pre as [??? [pre [[]]%termPiCongAlg_prem0%dup]%dup].
+      split ; [easy|..].
+      intros [|] Hty ? ; cbn in *.
+      2:now intros []%prod_tm_inj.
+      eapply implem_conv_graph, algo_conv_sound in Hty ; tea.
+      eapply dup in pre as [pre ?%termPiCongAlg_prem1] ; tea.
+      split ; [easy|..].
+      intros [|] ? Hty' ; [easy|..].
+      intros []%prod_tm_inj.
+      eapply Hty', stability1 ; tea.
       now econstructor.
-    + intros Hty'.
+      
+    - destruct s.
+      destruct pre as [??? [pre [[]]%termSigCongAlg_prem0%dup]%dup].
+      split ; [easy|..].
+      intros [|] Hty ? ; cbn in *.
+      2:now intros []%sig_tm_inj.
+      eapply implem_conv_graph, algo_conv_sound in Hty ; tea.
+      eapply dup in pre as [pre ?%termSigCongAlg_prem1] ; tea.
+      split ; [easy|..].
+      intros [|] ? Hty' ; [easy|..].
+      now intros []%sig_tm_inj.
+
+    - destruct s.
+      destruct pre as [??? [pre [[]]%termIdCongAlg_prem0%dup]%dup].
+      split ; [easy|..].
+      intros [|] Hty ? ; cbn in *.
+      2:now intros []%id_tm_inj.
+      eapply implem_conv_graph, algo_conv_sound in Hty ; tea.
+      eapply dup in pre as [pre [? []]%termIdCongAlg_prem1%dup] ; tea.
+      split ; [easy|..].
+      intros [|] Hty'%implem_conv_graph ? ; cbn in *.
+      2: now intros []%id_tm_inj.
+      eapply dup in Hty' as [Hty' ?%algo_conv_sound] ; tea.
+      eapply dup in pre as [pre ?%termIdCongAlg_prem2] ; tea.
+      split ; [easy|..].
+      intros [|] ? Hty'' ; cbn in * ; [easy|..].
+      now intros []%id_tm_inj.
+
+    - destruct pre as [??? [pre [[]]%termNeuConvAlg_prem0%dup]%dup] ; tea.
+      eapply whnf_view3_ty_neutral_can in e as [?%not_can_whne ?%not_can_whne] ; tea.
+      split ; [now split|..].
+      intros [|] ? Hty ; cbn ; [easy|..].
+      
+      destruct s.
+      unshelve eintros ?%conv_neu_conv_p ; eauto.
+      gen_typing.
+
+    - destruct s.
+      destruct pre as [_ wt wu [Ht Hu]].
+      eapply wft_term, type_isType in Ht, Hu ; tea.
+      unshelve eapply univ_mismatch_hd_view in e ; tea.
+      unshelve eintros H_view%univ_conv_inj ; tea.
+      rewrite e in H_view.
+      eassumption.
+
+    - destruct pre as [??? [pre [[]]%termFunConvAlg_prem2%dup]%dup] ; tea.
+      split ; [easy|..].
+      intros [|] ? Hty ; cbn ; [easy|..].
+
+      intros Hty'.
       eapply Hty.
       eapply convtm_meta_conv.
       3: reflexivity.
       1: econstructor.
-      1: erewrite <- !Weakening.wk1_ren_on.
+      1: erewrite <- !wk1_ren_on.
       1: eapply convtm_meta_conv.
       1: eapply convtm_wk ; tea.
-      * boundary.
-      * cbn ; reflexivity.
-      * reflexivity.
-      * eapply convtm_meta_conv.
+      + boundary.
+      + cbn ; reflexivity.
+      + reflexivity.
+      + eapply convtm_meta_conv.
         1: do 2 econstructor.
         1: boundary.
         constructor.
-        all: now Weakening.bsimpl.
-      * Weakening.bsimpl ; refold.
+        all: now bsimpl.
+      + bsimpl ; refold.
         rewrite scons_eta'.
-        now Weakening.bsimpl.
+        now bsimpl.
     
-  - now econstructor.
-  
-  - destruct pre as [??? [pre [[]]%termSuccCongAlg_prem0%dup]%dup] ; tea.
-    split ; [easy|..].
-    intros [|] Hty ; cbn.
-    + now econstructor.
-    + unshelve eintros ?%nat_conv_inj.
+    - destruct pre as [??? [pre [[]]%termSuccCongAlg_prem0%dup]%dup] ; tea.
+      split ; [easy|..].
+      intros [|] ? Hty ; cbn in * ; [easy|..].
+      unshelve eintros ?%nat_conv_inj.
       1-2: now constructor.
       cbn in *.
       eauto.
-      
-  - destruct pre as [??? [pre [[]]%termPairConvAlg_prem2%dup]%dup] ; tea.
-    split ; [easy|..].
-    intros [|] ; cbn.
-    + eintros [ Hpost%algo_conv_sound]%dup ; tea.
-      eapply termPairConvAlg_prem3 in Hpost ; tea.
+        
+    - destruct pre as [??? [pre [[]]%termPairConvAlg_prem2%dup]%dup] ; tea.
       split ; [easy|..].
-      intros [|].
-      1: now econstructor.
-      intros Hnty Hty.
-      eapply Hnty.
-      now econstructor.
-    + intros Hnty Hty.
-      eapply Hnty.
-      now econstructor.
-  
-  - now econstructor.
-  
-  - destruct pre as [??? [pre [[]]%termNeuConvAlg_prem0%dup]%dup] ; tea.
-    split ; [easy|..].
-    eapply whnf_view3_neutrals_can in e as [Wa Wn Wn'].
-    2: easy.
-    intros [|] ; cbn.
-    + now econstructor.
-    + intros Hnty Hty.
-      eapply whne_can in Wn, Wn' ; eauto.
+      intros [|] ; cbn in *.
+      + eintros Hpost ? ; tea.
+        eapply implem_conv_graph, algo_conv_sound in Hpost ; tea.
+        eapply termPairConvAlg_prem3 in Hpost ; tea.
+        split ; [easy|..].
+        intros [|].
+        1: now econstructor.
+        intros ? Hnty Hty.
+        eapply Hnty.
+        now econstructor.
+      + intros ? Hnty Hty.
+        eapply Hnty.
+        now econstructor.
+    
+    - destruct pre as [??? [pre [[]]%termNeuConvAlg_prem0%dup]%dup] ; tea.
+      eapply whnf_view3_neutrals_can in e as [Wa Wn Wn'] ; tea.
+      split.
+      1: split ; tea ; eauto using not_can_whne.
+      intros [|] ; cbn ; [easy|..].
+      intros ? Hnty Hty.
+      eapply not_can_whne in Wn, Wn' ; eauto.
       eapply Hnty.
       exists A.
-      destruct Wa.
-      * destruct s.
-        unshelve eapply univ_conv_inj in Hty.
-        1-2: now econstructor.
-        now cbn in *.
-      * unshelve eapply nat_conv_inj in Hty.
-        1-2: now econstructor.
-        now cbn in *.
-      * unshelve eapply empty_conv_inj in Hty.
-        all: now cbn in *.
-      * unshelve eapply id_conv_inj in Hty.
-        1-2: now econstructor.
-        now cbn in *.
-      * now eapply neu_conv_inj in Hty.
-  
-  - destruct pre as [w ?? []].
-    eapply type_isType in w.
-    2: boundary.
-    unshelve eapply mismatch_hd_view in e as [(?&?&[->])|(?&?&?&?&?&[->])] ; tea.
-    + unshelve eintros ?%nat_conv_inj ; tea.
-      now rewrite e in H.
+      now eapply conv_neu_conv_p.
+    
+    - destruct pre as [w ?? []].
+      eapply type_isType in w.
+      2: boundary.
+      unshelve eapply mismatch_hd_view in e as [(?&?&[->])|(?&?&?&?&?&[->])] ; tea.
+      + unshelve eintros ?%nat_conv_inj ; tea.
+        now rewrite e in H.
 
-    + unshelve eintros ?%id_conv_inj ; tea.
-      now rewrite e in H.
+      + unshelve eintros ?%id_conv_inj ; tea.
+        now rewrite e in H.
 
-  - destruct (Nat.eqb_spec n n') ; cbn.
-    + destruct pre as [_ [? [? [(?& []) ?]]%termGen']] ; subst.
-      erewrite ctx_access_complete ; cbn.
-      1: econstructor.
-      all: eassumption.
+    - destruct (Nat.eqb_spec n n') ; cbn.
+      + destruct pre as [[] [_ [? [? [(?& []) ?]]%termGen']]] ; subst.
+        erewrite ctx_access_complete ; cbn.
+        1: econstructor.
+        all: eassumption.
+        
+      + intros [? (?&[[= ->]])%neuConvGen].
+        eauto.
       
-    + intros [? (?&[[= ->]])%neuConvGen].
-      eauto.
-    
-  - apply dup in pre as [pre [[] ]%neuAppCongAlg_prem0%dup] ; eauto.
-    split ; [easy|..].
-    intros [|] ; cbn.
-    + intros [[Hpost]%dup] ; tea.
-      eapply algo_conv_sound in Hpost as [Hconv Hfu ?] ; tea.
-      eapply dup in pre as [pre [[? (?&[? [? [-> Hf]]]&?)%termGen'] _]].
-      eapply Hfu, red_compl_prod_r in Hf as (?&?&[red%redty_sound]).
-      eapply red_whnf in red ; eauto ; subst.
-      edestruct neuAppCongAlg_prem1 ; eauto.
+    - destruct pre as [[wn wn'] [pre [[] ]%neuAppCongAlg_prem0%dup]%dup] ; eauto.
+      inversion wn ; inversion wn' ; subst.
+      split ; [easy|..].
+      intros [|] ; cbn in *.
+      + intros [Hpost]%implem_conv_graph ; tea ; refold.
+        eapply algo_conv_sound in Hpost as [Hconv Hfu ?] ; tea.
+        eapply dup in pre as [pre [[? (?&[? [? [-> Hf]]]&?)%termGen'] _]].
+        eapply Hfu, red_compl_prod_r in Hf as (?&?&[red%redty_sound]).
+        eapply red_whnf in red ; eauto ; subst.
+        edestruct neuAppCongAlg_prem1 ; eauto.
 
+        cbn.
+        split ; [eauto|..].
+        intros [|] ? ; cbn in * ; [easy|..].
+
+        intros Hneg [? (?&?&?&?&[[=]])%neuConvGen] ; subst.
+        apply Hneg.
+        eapply TermConv ; refold ; tea.
+        eapply prod_ty_inj, Hfu.
+        eauto using conv_neu_sound with boundary.
+
+      + intros ? Hneg [? (?&?&?&?&[[=]])%neuConvGen] ; subst.
+        apply Hneg.
+        eexists ; split ; eauto.
+        now constructor.
+  
+    - destruct pre as [[wn wn'] [pre [[] ]%neuNatElimCong_prem0%dup]%dup] ; eauto.
+      inversion wn ; inversion wn' ; subst.
+      split ; [easy|..].
+      intros [|] ; cbn in *.
+      2: shelve.
+
+      intros [Hpost]%implem_conv_graph ; tea.
+      eapply algo_conv_sound in Hpost as [Hconv Hfu ?] ; tea.
+      eapply dup in pre as [pre [[? (?&[-> ??? Hn]&?)%termGen'] _]].
+      eapply Hfu, red_compl_nat_r, redty_sound, red_whnf in Hn ; eauto ; subst.
+      eapply dup in pre as [pre [ []]%neuNatElimCong_prem1%dup] ; eauto.
       cbn.
-      split ; [eauto|..].
+      split ; [easy|..].
       intros [|] ; cbn.
-      1: now econstructor.
+      2: shelve.
 
-      intros Hneg [? (?&?&?&?&[[=]])%neuConvGen] ; subst.
-      apply Hneg.
-      eapply TermConv ; refold ; tea.
-      eapply prod_ty_inj, Hfu.
-      eauto using conv_neu_sound with boundary.
+      eintros [Hpost1]%implem_conv_graph%algo_conv_sound%dup ; tea ; cbn in *.
+      eapply neuNatElimCong_prem2, dup in Hpost1 as [Hpost1 []] ; eauto.
+      split ; [easy|..].
+      intros [|] ; cbn.
+      2: shelve.
+      
+      intros [Hpost2]%implem_conv_graph%algo_conv_sound%dup ; tea.
+      eapply neuNatElimCong_prem3, dup in Hpost2 as [Hpost2 []] ; eauto.
+      split ; [easy|..].
+      intros [|] ; cbn ; [easy|..].
 
-    + intros Hneg [? (?&?&?&?&[[=]])%neuConvGen] ; subst.
-      apply Hneg.
-      eexists ; split ; eauto.
-      now constructor.
- 
-  - apply dup in pre as [pre [[] ]%neuNatElimCong_prem0%dup] ; eauto.
-    split ; [easy|..].
-    intros [|] ; cbn.
-    2: shelve.
-
-    intros [[Hpost]%dup] ; tea.
-    eapply algo_conv_sound in Hpost as [Hconv Hfu ?] ; tea.
-    eapply dup in pre as [pre [[? (?&[-> ??? Hn]&?)%termGen'] _]].
-    eapply Hfu, red_ty_compl_nat_r, redty_sound, red_whnf in Hn ; eauto ; subst.
-    eapply dup in pre as [pre [ []]%neuNatElimCong_prem1%dup] ; eauto.
-    cbn.
-    split ; [easy|..].
-    intros [|] ; cbn.
-    2: shelve.
-
-    intros [? [Hpost1 ?]%algo_conv_sound%dup]%dup ; tea.
-    eapply neuNatElimCong_prem2, dup in Hpost1 as [Hpost1 []] ; eauto.
-    split ; [easy|..].
-    intros [|] ; cbn.
-    2: shelve.
-    
-    intros [? [Hpost2 ?]%algo_conv_sound%dup]%dup ; tea.
-    eapply neuNatElimCong_prem3, dup in Hpost2 as [Hpost2 []] ; eauto.
-    split ; [easy|..].
-    intros [|] ; cbn.
-    2: shelve.
-    
-    intros.
-    now econstructor.
-
-    Unshelve.
-    all: intros Hneg [? (?&?&?&?&[[= <- <- <-]])%neuConvGen] ; subst.
-    all: apply Hneg ; eauto.
-    eexists ; split ; gen_typing.
-  
-  - apply dup in pre as [pre [[] ]%neuEmptyElimCong_prem0%dup] ; eauto.
-    split ; [easy|..].
-    intros [|] ; cbn.
-    2: shelve.
-
-    intros [[Hpost]%dup] ; tea.
-    eapply algo_conv_sound in Hpost as [Hconv Hfu ?] ; tea.
-    eapply dup in pre as [pre [[? (?&[-> ? Hn]&?)%termGen'] _]].
-    eapply Hfu, red_compl_empty_r, redty_sound, red_whnf in Hn ; eauto ; subst.
-    eapply dup in pre as [pre [ []]%neuEmptyElimCong_prem1%dup] ; eauto.
-    cbn.
-    split ; [easy|..].
-    intros [|] ; cbn.
-    2: shelve.
-    
-    intros.
-    now econstructor.
-
-    Unshelve.
-    all: intros Hneg [? (?&?&[[=]])%neuConvGen] ; subst.
-    all: apply Hneg ; eauto.
-    eexists ; split ; gen_typing.
-  
-  - apply dup in pre as [pre [[] ]%neuFstCongAlg_prem0%dup] ; eauto.
-    split ; [easy|..].
-    intros [|] ; cbn.
-    
-    + intros [[Hpost]%dup] ; tea.
-      eapply algo_conv_sound in Hpost as [Hconv Hfu ?] ; tea.
-      eapply dup in pre as [pre [[? (?&(?&?&->&Hp)&?)%termGen'] _]].
-      eapply Hfu, red_compl_sig_r in Hp as (?&?&[red%redty_sound]).
-      eapply red_whnf in red ; eauto ; subst.
-      cbn.
-      now econstructor.
-
-    + intros Hneg [? (?&?&?&[[= <-]])%neuConvGen].
-      eapply Hneg.
+      Unshelve.
+      all: intros ? Hneg [? (?&?&?&?&[[= <- <- <-]])%neuConvGen] ; subst.
+      all: apply Hneg ; eauto.
       eexists ; split ; gen_typing.
-  
-  - apply dup in pre as [pre [[] ]%neuSndCongAlg_prem0%dup] ; eauto.
-    split ; [easy|..].
-    intros [|] ; cbn.
     
-    + intros [[Hpost]%dup] ; tea.
+    - destruct pre as [[wn wn'] [pre [[] ]%neuEmptyElimCong_prem0%dup]%dup] ; eauto.
+      inversion wn ; inversion wn' ; subst.
+      split ; [easy|..].
+      intros [|] ; cbn.
+      2: shelve.
+
+      intros [Hpost]%implem_conv_graph ; tea.
       eapply algo_conv_sound in Hpost as [Hconv Hfu ?] ; tea.
-      eapply dup in pre as [pre [[? (?&(?&?&->&Hp)&?)%termGen'] _]].
-      eapply Hfu, red_compl_sig_r in Hp as (?&?&[red%redty_sound]).
-      eapply red_whnf in red ; eauto ; subst.
+      eapply dup in pre as [pre [[? (?&[-> ? Hn]&?)%termGen'] _]].
+      eapply Hfu, red_compl_empty_r, redty_sound, red_whnf in Hn ; eauto ; subst.
+      eapply dup in pre as [pre [ []]%neuEmptyElimCong_prem1%dup] ; eauto.
       cbn.
-      now econstructor.
+      split ; [easy|..].
+      intros [|] ; cbn ; [easy|..].
 
-    + intros Hneg [? (?&?&?&[[= <-]])%neuConvGen].
-      eapply Hneg.
+      Unshelve.
+      all: intros ? Hneg [? (?&?&[[=]])%neuConvGen] ; subst.
+      all: apply Hneg ; eauto.
       eexists ; split ; gen_typing.
-  
-  - apply dup in pre as [pre [[] ]%neuIdElimCong_prem0%dup] ; eauto.
-    split ; [easy|..].
-    intros [|] ; cbn.
-    2: shelve.
-
-    intros [[Hpost]%dup] ; tea.
-    eapply algo_conv_sound in Hpost as [Hconv Hfu ?] ; tea.
-    eapply dup in pre as [pre [[? (?&[-> ????? He]&?)%termGen'] _]].
-    eapply Hfu, red_compl_id_r in He as (?&?&?&[red%redty_sound]).
-    eapply red_whnf in red ; eauto ; subst.
-    eapply dup in pre as [pre [ []]%neuIdElimCong_prem1%dup] ; eauto.
-    cbn.
-    split ; [erewrite <- !wk1_ren_on ; easy|..].
-    intros [|] ; cbn.
-    2: shelve.
-
-    intros [? ?%algo_conv_sound%dup]%dup.
-    2-3: now erewrite <- !wk1_ren_on.
-    eapply neuIdElimCong_prem2 in pre ; eauto.
-    2: now rewrite !wk1_ren_on.
-    split ; [easy|..].
-    intros [|] ; cbn.
-    2: shelve.
-    econstructor ; eauto.
-    now rewrite !wk1_ren_on.
-
-    Unshelve.
-    all: intros Hneg [? (?&?&?&?&?&?&[[= <- <- <-]])%neuConvGen] ; subst.
-    all: apply Hneg ; eauto.
-    + eexists ; split ; gen_typing.
-    + now erewrite <- !wk1_ren_on. 
     
-  
-  - intros [? ?%neuConvGen].
-    destruct t ; cbn in * ; try solve [easy].
-    all: prod_hyp_splitter ; subst.
-    all: simp build_ne_view2 in e ; cbn in *.
-    all: congruence.
-  
-  - split ; [easy|..].
-    intros [|] Hty ; cbn.
-    + intros ? []%red_sound ; split ; tea.
-      now econstructor.
-    + intros [? []].
+    - destruct pre as [[wn wn'] [pre [[] ]%neuFstCongAlg_prem0%dup]%dup] ; eauto.
+      inversion wn ; inversion wn' ; subst.
+      split ; [easy|..].
+      intros [|] ; cbn.
+      
+      + intros [Hpost]%implem_conv_graph ; tea.
+        eapply algo_conv_sound in Hpost as [Hconv Hfu ?] ; tea.
+        eapply dup in pre as [pre [[? (?&(?&?&->&Hp)&?)%termGen'] _]].
+        eapply Hfu, red_compl_sig_r in Hp as (?&?&[red%redty_sound]).
+        eapply red_whnf in red ; eauto ; subst.
+        now cbn.
+
+      + intros ? Hneg [? (?&?&?&[[= <-]])%neuConvGen].
+        eapply Hneg.
+        eexists ; split ; gen_typing.
+    
+    - destruct pre as [[wn wn'] [pre [[] ]%neuSndCongAlg_prem0%dup]%dup] ; eauto.
+      inversion wn ; inversion wn' ; subst.
+      split ; [easy|..].
+      intros [|] ; cbn.
+      
+      + intros [Hpost]%implem_conv_graph ; tea.
+        eapply algo_conv_sound in Hpost as [Hconv Hfu ?] ; tea.
+        eapply dup in pre as [pre [[? (?&(?&?&->&Hp)&?)%termGen'] _]].
+        eapply Hfu, red_compl_sig_r in Hp as (?&?&[red%redty_sound]).
+        eapply red_whnf in red ; eauto ; subst.
+        now cbn.
+
+      + intros ? Hneg [? (?&?&?&[[= <-]])%neuConvGen].
+        eapply Hneg.
+        eexists ; split ; gen_typing.
+    
+    - destruct pre as [[wn wn'] [pre [[] ]%neuIdElimCong_prem0%dup]%dup] ; eauto.
+      inversion wn ; inversion wn' ; subst.
+      split ; [easy|..].
+      intros [|] ; cbn.
+      2: shelve.
+
+      intros [Hpost]%implem_conv_graph ; tea.
+      eapply algo_conv_sound in Hpost as [Hconv Hfu ?] ; tea.
+      eapply dup in pre as [pre [[? (?&[-> ????? He]&?)%termGen'] _]].
+      eapply Hfu, red_compl_id_r in He as (?&?&?&[red%redty_sound]).
+      eapply red_whnf in red ; eauto ; subst.
+      eapply dup in pre as [pre [ []]%neuIdElimCong_prem1%dup] ; eauto.
+      cbn.
+      split ; [erewrite <- !wk1_ren_on ; easy|..].
+      intros [|] ; cbn.
+      2: shelve.
+
+      intros []%implem_conv_graph%algo_conv_sound%dup.
+      2-3: now erewrite <- !wk1_ren_on.
+      eapply neuIdElimCong_prem2 in pre ; eauto.
+      2: now rewrite !wk1_ren_on.
+      split ; [easy|..].
+      intros [|] ; cbn ; [easy|..].
+
+      Unshelve.
+      all: intros ? Hneg [? (?&?&?&?&?&?&[[= <- <- <-]])%neuConvGen] ; subst.
+      all: apply Hneg ; eauto.
+      + eexists ; split ; gen_typing.
+      + now erewrite <- !wk1_ren_on. 
+
+    - intros [? ?%neuConvGen].
+      destruct t ; cbn in * ; try solve [easy].
+      all: prod_hyp_splitter ; subst.
+      all: simp build_ne_view2 in e ; cbn in *.
+      all: congruence.
+    
+    - split ; [easy|..].
+      intros [|] ? Hty ; cbn ; [easy|..].
+      intros [? []].
       now eapply Hty.
 
-Qed.
+  Qed.
+
+End ConvSoundNeg.
