theories/Syntax/Notations.v
@@ -34,7 +34,7 @@ Class ConvTerm (ta : tag) := conv_term : context -> term -> term -> term -> Set.
 Class ConvTermRed (ta : tag) := conv_term_red : context -> term -> term -> term -> Set.
 Class ConvNeu (ta : tag) := conv_neu : context -> term -> term -> term -> Set.
 Class ConvNeuRed (ta : tag) := conv_neu_red : context -> term -> term -> term -> Set.
-Class ConvNeuConv (ta : tag) := conv_neu_conv : context -> term -> term -> term -> Set.
+Class ConvNeuConv (ta : tag) := conv_neu_ty : context -> term -> term -> term -> Set.
 
 (** The context Γ is well-formed *)
 Notation "[ |- Γ ]" := (wf_context Γ)
@@ -94,9 +94,9 @@ Notation "[ Γ |-[ ta  ] n ~ n' ▹ A ]" := (conv_neu (ta := ta) Γ A n n')
 Notation "[ Γ |- n '~h' n' ▹ A ]" := (conv_neu_red Γ A n n') (at level 0, Γ, n, n', A at level 50, only parsing) : typing_scope.
 Notation "[ Γ |-[ ta  ] n '~h' n' ▹ A ]" := (conv_neu_red (ta := ta) Γ A n n') (at level 0, ta, Γ, n, n', A at level 50) : typing_scope.
 (** Neutral n and n' are convertible in Γ at type A *)
-Notation "[ Γ |- n ~ n' : A ]" := (conv_neu_conv Γ A n n')
+Notation "[ Γ |- n ~ n' : A ]" := (conv_neu_ty Γ A n n')
   (at level 0, Γ, n, n', A at level 50, only parsing) : typing_scope. 
-Notation "[ Γ |-[ ta  ] n ~ n' : A ]" := (conv_neu_conv (ta := ta) Γ A n n')
+Notation "[ Γ |-[ ta  ] n ~ n' : A ]" := (conv_neu_ty (ta := ta) Γ A n n')
   (at level 0, ta, Γ, n, n', A at level 50) : typing_scope.
 
 (** ** Untyped Conversion *)
